lazy_list/code.v
@@ -86,20 +86,20 @@ Module LazyList (Params: LAZY_LIST_PARAMS).
       let: "ck" := (nodeKey "curr") in
       if: "k" = "ck"
       then
-        release (nodeLock "pred");;
-        #false
+        release (nodeLock "pred")
+        (* ;; #false *)
       else
         match: nodeNext "pred" with
             NONE =>
-            release (nodeLock "pred");;
-            #false
+            release (nodeLock "pred")
+            (* ;; #false *)
           | SOME "np" =>
             let: "succ" := !"np" in
             let: "next" := ref "succ" in
             let: "node" := ("k", SOME "next", newlock #()) in
             "np" <- "node";;
-            release (nodeLock "pred");;
-            #true
+            release (nodeLock "pred")
+            (* ;; #true *)
         end.
 
 End LazyList.
