lazy_list/spec.v
@@ -10,13 +10,13 @@ Module LazyListSpec (Params: LAZY_LIST_PARAMS).
   Import Invariant.
 
   Section Proofs.
-    Context `{!heapGS Σ, lockG Σ} (N : namespace).
+    Context `{!heapGS Σ, !gset_list_unionGS Σ, lockG Σ} (N : namespace).
 
     Theorem new_spec :
       {{{ True }}}
         new #()
-      {{{ v, RET v; 
-        is_lazy_list N ∅ v 
+      {{{ Γ v, RET v; 
+        is_lazy_list N v ∅ 1 Γ
       }}}.
     Proof.
       iIntros (Φ) "_ HΦ".
@@ -27,21 +27,30 @@ Module LazyListSpec (Params: LAZY_LIST_PARAMS).
       iIntros (l) "#Hlock". iDestruct "Hlock" as (γ) "Hlock".
       set (head := (INT_MIN, Some t, l)).
       wp_pures; rewrite (fold_rep_to_node head).
-      iMod (inv_alloc N ⊤ (lazy_list_inv ∅ head) with "[Ht2 Hlock]") as "Hinv".
-      + iNext. iExists nil.
-        iSplit. done. iSplit. simpl. 
-        assert (node_lt head tail) as Hlt.
-        { unfold node_lt; unfold node_key; simpl; apply HMIN_MAX. }
-        auto using Hlt.
-        iExists t, γ. iFrame "#". by iFrame.
-      + iApply "HΦ". iExists head, ∅. iModIntro.
-        iSplit. by unfold key_equiv.
+
+      iMod (own_alloc (● (∅ : gset node_rep) ⋅ ◯ (∅: gset node_rep)))
+        as (γauth) "[Hown_auth Hown_auth_frag]"; first by apply auth_both_valid.
+      iMod (own_alloc (●F (∅ : gset node_rep) ⋅ ◯F (∅: gset node_rep)))
+        as (γfrac) "[Hown_frac Hown_frac_frag]"; first by apply auth_both_valid.
+
+      iMod (inv_alloc N ⊤ (lazy_list_inv head γauth γfrac) 
+        with "[Ht2 Hlock Hown_auth Hown_frac]") as "#Hinv".
+      + iNext. iExists ∅, nil. iFrame.
+        iSplit. done. iSplit. 
+        assert (node_lt head tail); last (simpl; auto).
+        { rewrite /node_lt/node_key//=; apply HMIN_MAX. }
+        iExists t, γ. by iFrame "# ∗".
+      + iModIntro; iApply ("HΦ" $! (mk_lazy_gname γauth γfrac)).
+        iExists head, ∅.
+        iSplit; first by unfold key_equiv.
         by (repeat iSplit).
     Qed.
     
-    Theorem find_spec (head curr: node_rep) (key: Z) (S: gset node_rep) :
+    Theorem find_spec1 (head curr: node_rep) (key: Z) (S: gset node_rep) (γs γf: gname) :
       {{{ 
-        inv N (lazy_list_inv S head)
+        inv N (lazy_list_inv head γs γf)
+        ∗
+        own γf (◯F S)
         ∗
         ⌜ curr = head ∨ curr ∈ S ⌝
         ∗
@@ -49,37 +58,31 @@ Module LazyListSpec (Params: LAZY_LIST_PARAMS).
       }}}
       find (rep_to_node curr) #key
       {{{ pred succ, RET SOMEV ((rep_to_node pred), (rep_to_node succ));
-        ⌜ node_key pred < key ≤ node_key succ ⌝
-        ∗
-        ⌜ pred = head ∨ pred ∈ S ⌝
-        ∗
-        ⌜ succ ∈ S ∨ succ = tail ⌝
+        own γf (◯F S)
         ∗
         ⌜ key ∈ map node_key (elements S) ↔ node_key succ = key ⌝
-        ∗
-        ∃ (l:loc) (γ: gname), ⌜ node_next pred = Some l ⌝ 
-                              ∗ 
-                              is_lock γ (node_lock pred) (node_inv l)
       }}}.
     Proof.
-      iIntros (Φ) "(#Hinv & Hcurr_range & Hrange) HΦ".
-      iRevert (curr) "Hcurr_range Hrange HΦ".
-      iLöb as "IH". 
-      iIntros (curr) "%Hcurr_range %Hrange HΦ".
+      iIntros (Φ) "(#Hinv & Hown_frag & Hcurr_range & Hrange) HΦ".
+      iRevert (curr) "Hown_frag Hcurr_range Hrange HΦ".
+      iLöb as "IH".
+      iIntros (curr) "Hown_frag %Hcurr_range %Hrange HΦ".
       wp_lam. wp_let. wp_lam. wp_pures.
 
       destruct (node_next curr) as [l|] eqn:Hcurr_next; wp_pures.
       + wp_bind (Load _).
-        iInv N as (L) "(>%Hperm & >%Hsort & Hlist)" "Hclose".
+        iInv N as (S' L) "(>%Hperm & >%Hsort & Hown_auth & Hown_frac & Hlist)" "Hclose".
+        iMod "Hown_frac"; iDestruct (own_valid_2 with "Hown_frac Hown_frag") 
+          as %->%frac_auth_agree_L.
 
         edestruct (in_split curr ([head] ++ L)) as (Ls&Lf&Hcurr).
         { destruct Hcurr_range; first by left.
-          right. apply elem_of_list_In. rewrite Hperm. apply elem_of_elements; auto. }
+          by right; rewrite -elem_of_list_In Hperm elem_of_elements. }
   
-        edestruct (node_rep_split_join Lf curr key) as (pred&succ&L1&L2&?&Hsplit_join).
-        { split; lia. }
+        edestruct (node_rep_split_join Lf curr key) as (pred&succ&L1&L2&?&Hsplit_join); auto.
   
-        feed pose proof (node_rep_split_sep L Ls Lf L1 L2 head curr pred succ key) as Htemp; eauto; try lia.
+        feed pose proof (node_rep_split_sep L Ls Lf L1 L2 head curr pred succ key) 
+          as Htemp; auto.
         destruct Htemp as [Lm Hsplit_sep].
 
         destruct Lm as [|next Lm].
@@ -89,80 +92,61 @@ Module LazyListSpec (Params: LAZY_LIST_PARAMS).
           assert (l = l') as <- by congruence.
 
           wp_load.
-          iMod ("Hclose" with "[Hpt Himp]").
+          iMod ("Hclose" with "[Hpt Himp Hown_auth Hown_frac]").
           {
-            iNext. iExists L.
-            iSplit. done.
-            iSplit. done.
-            iApply "Himp". iFrame.
+            iNext. iExists S, L.
+            iPoseProof ("Himp" with "Hpt") as "Hlist".
+            by iFrame.
           }
-          iModIntro. wp_let. wp_lam. wp_pures.
 
+          iModIntro. wp_let. wp_lam. wp_pures.
           case_bool_decide; last lia.
           wp_pures. iApply "HΦ".
-          iModIntro.
-
-          iSplit; first by (iPureIntro; lia).
-          iSplit; first by (iPureIntro; auto).
-          iSplit.
-          { 
-            iPureIntro. rewrite -elem_of_elements. rewrite -Hperm.
-            rewrite elem_of_list_In. apply in_inv_rev.
-            destruct Ls.
-            ++ inversion Hsplit_sep. by left.
-            ++ inversion Hsplit_sep. apply in_app_iff.
-               right. right; left. auto.
-          }
-
-          iSplit; last first.
-          { iExists l, γ. by iFrame "#". }
+          iModIntro; iFrame.
 
           iPureIntro.
-          rewrite -Hperm. split; intros.
+          rewrite -Hperm; split; intros.
           * eapply (sorted_node_lt_cover_gap (Ls ++ L1) L2 pred); try lia.
             ++ by rewrite app_ass -Hsplit_join //= app_comm_cons -app_ass -Hcurr app_ass.
-            ++ cut (In key (map node_key ([head] ++ L ++ [tail]))).
-               -- intros Hin. 
-                  rewrite -app_ass Hcurr app_ass in Hin.
-                  by rewrite app_ass -Hsplit_join.
-               -- rewrite -app_ass map_app.
-                  apply in_app_iff. left. right. 
-                  by apply elem_of_list_In.
-          * apply elem_of_list_In. apply in_map_iff. exists succ; split; auto.
+            ++ assert (In key (map node_key ([head] ++ L ++ [tail]))) as Hin.
+               { rewrite -app_ass map_app in_app_iff; left; right. 
+                 by apply elem_of_list_In. }
+               rewrite -app_ass Hcurr app_ass in Hin.
+               by rewrite app_ass -Hsplit_join.
+          * rewrite elem_of_list_In in_map_iff. exists succ; split; auto.
             cut (In succ Lf).
-            { 
-              destruct Ls; inversion Hcurr; subst; auto.
-              intros. rewrite in_app_iff. right. by right.
-            }
+            { destruct Ls; inversion Hcurr; subst; auto.
+              intros; by rewrite in_app_iff; right; right. }
+
             cut (In succ (Lf ++ [tail])).
-            { 
-              rewrite /tail.
-              rewrite ?in_app_iff. intros [|[|[]]]; auto; subst. 
-              unfold node_key in Hrange. simpl in Hrange. lia.
-            }
+            { rewrite /tail ?in_app_iff.
+              intros [|[|[]]]; auto; subst. 
+              unfold node_key in Hrange. simpl in Hrange; lia. }
 
             destruct L1.
-            ** rewrite //= in Hsplit_join. inversion Hsplit_join as [[Heq1 Heq2]]; subst.
-              rewrite Heq2. by left.
-            ** inversion Hsplit_join as [[Heq1 Heq2]]; subst. rewrite Heq2.
-              rewrite in_app_iff. right. right. left. auto.
+            ** rewrite //= in Hsplit_join. 
+               inversion Hsplit_join as [[Heq1 Heq2]]; subst.
+               by rewrite Heq2; left.
+            ** inversion Hsplit_join as [[Heq1 Heq2]]; subst.
+               by rewrite Heq2 in_app_iff; right; right; left.
         - rewrite (list_equiv_split curr next ([head] ++ L)); last first.
           { simpl in *. by rewrite -Hsplit_sep. }
           iDestruct "Hlist" as (l' γ) "(>%Hsome & Hpt & #Hlock & Himp)".
           assert (l = l') as <- by congruence.
-          wp_load.
-          iMod ("Hclose" with "[Hpt Himp]").
-          {
-            iNext. iExists L.
-            iSplit. done.
-            iSplit. done.
-            iApply "Himp". iFrame.
-          }
-          iModIntro. wp_let. wp_lam. wp_pures.
 
+          wp_load.
+          iMod ("Hclose" with "[Hpt Himp Hown_auth Hown_frac]").
+          {
+            iNext. iExists S, L.
+            iPoseProof ("Himp" with "Hpt") as "Hlist".
+            by iFrame.
+          }
+
+          iModIntro. wp_let. wp_lam. wp_pures.
           case_bool_decide as Hcase.
           * exfalso.
-            cut (node_key next <= node_key pred); first by lia.
+            assert (node_key next <= node_key pred); last by lia.
+
             assert (In pred (next :: Lm)) as Hpred_in_m.
             {
               symmetry in Hsplit_sep.
@@ -181,110 +165,185 @@ Module LazyListSpec (Params: LAZY_LIST_PARAMS).
                  rewrite app_ass //= in Hsplit_sep.
                  rewrite //= app_ass app_ass //=.
             }
-            cut (Sorted node_lt ([next] ++ Lm)).
-            -- intros Hsort'.
-               apply Sorted_StronglySorted in Hsort'; last first.
-               { unfold Relations_1.Transitive; apply node_lt_transitive. } 
-               inversion Hsort'; subst. 
-               inversion Hpred_in_m; first by (subst; lia).
-               apply node_lt_le_incl.
-               eapply Forall_forall; eauto.
-               rewrite elem_of_list_In //=.
-            -- rewrite -Hsplit_sep in Hsort.
-               by repeat (apply node_rep_sorted_app in Hsort as (? & Hsort)).
+
+            assert (Sorted node_lt ([next] ++ Lm)) as Hsort'.
+            { rewrite -Hsplit_sep in Hsort.
+              by repeat (apply node_rep_sorted_app in Hsort as (? & Hsort)). }
+
+            apply Sorted_StronglySorted in Hsort'; last first.
+            { unfold Relations_1.Transitive; apply node_lt_transitive. } 
+            inversion Hsort'; subst. 
+            inversion Hpred_in_m; first by (subst; lia).
+            eapply node_lt_le_incl, Forall_forall; eauto.
+            rewrite elem_of_list_In //=.
           * wp_if.
-            iApply ("IH" $! next with "[%] [%]").
+            iApply ("IH" $! next with "[Hown_frag] [%] [%]").
+            { iFrame. }
             { 
-              right. apply elem_of_elements. rewrite -Hperm.
+              right. rewrite -elem_of_elements -Hperm.
               destruct Ls; assert (In next (L ++ [tail])) as Hin.
               -- inversion Hsplit_sep. by left.
               -- apply in_app_iff in Hin.
                  destruct Hin as [|[|[]]]; first by eapply elem_of_list_In.
-                 subst. exfalso. rewrite /node_key/tail//= in Hcase; lia.
-              -- inversion Hsplit_sep. apply in_app_iff.
-                 right. right; left. auto.
+                 subst; exfalso. 
+                 rewrite /node_key/tail//= in Hcase; lia.
+              -- inversion Hsplit_sep. 
+                 by apply in_app_iff; right; right; left.
               -- apply in_app_iff in Hin.
                  destruct Hin as [|[|[]]]; first by eapply elem_of_list_In.
-                 subst. exfalso. rewrite /node_key/tail//= in Hcase; lia.
+                 subst; exfalso. 
+                 rewrite /node_key/tail//= in Hcase; lia.
             }
             { lia. }
 
             iNext. iApply "HΦ".
-      + iInv N as (L) "(>%Hperm & >%Hsort & Hlist)" "Hclose".
+      + iInv N as (S' L) "(>%Hperm & >%Hsort & Hown_auth & Hown_frac & Hlist)" "Hclose".
+        iMod "Hown_frac"; iDestruct (own_valid_2 with "Hown_frac Hown_frag") 
+          as %->%frac_auth_agree_L.
 
-        edestruct (in_split curr ([head] ++ L)) as (Ls&Lf&Hcurr).
-        { destruct Hcurr_range; first by left.
-          right. apply elem_of_list_In. rewrite Hperm. apply elem_of_elements; auto. }
-  
-        edestruct (node_rep_split_join Lf curr key) as (pred&succ&L1&L2&?&Hsplit_join).
-        { split; lia. }
-  
-        feed pose proof (node_rep_split_sep L Ls Lf L1 L2 head curr pred succ key) as Htemp; eauto; try lia.
-        destruct Htemp as [Lm Hsplit_sep].
-
-        destruct Lm as [|next Lm].
-        - rewrite (list_equiv_split curr succ ([head] ++ L)); last first.
-          { simpl in *. by rewrite -Hsplit_sep. }
-          iDestruct "Hlist" as (? ?) "(>%Hsome & Hpt & #Hlock & Himp)".
-          iMod ("Hclose" with "[Hpt Himp]").
-          {
-            iNext. iExists L.
-            iSplit. done.
-            iSplit. done.
-            iApply "Himp". iFrame.
-          }
-          congruence.
-        - rewrite (list_equiv_split curr next ([head] ++ L)); last first.
-          { simpl in *. by rewrite -Hsplit_sep. }
-          iDestruct "Hlist" as (? ?) "(>%Hsome & Hpt & #Hlock & Himp)".
-          iMod ("Hclose" with "[Hpt Himp]").
-          {
-            iNext. iExists L.
-            iSplit. done.
-            iSplit. done.
-            iApply "Himp". iFrame.
-          }
-          congruence.
+        rewrite (list_equiv_invert); last first.
+        { by rewrite -elem_of_list_In Hperm elem_of_elements. }
+        iDestruct "Hlist" as (succ l γ) "(Hsucc_range & Hsome & Hpt & #Hlock & Himp)".
+        iMod "Hsome" as %Hsome; congruence.
     Qed.
     
-    Theorem contains_spec (v: val) (key: Z) (Skeys: gset Z)
+    Theorem contains_spec (v: val) (key: Z) (Skeys: gset Z) (Γ: lazy_gname)
       (Hrange: INT_MIN < key < INT_MAX) :
-      {{{ is_lazy_list N Skeys v }}}
+      {{{ is_lazy_list N v Skeys 1 Γ }}}
         contains v #key
       {{{ (b: bool), RET #b; 
-        is_lazy_list N Skeys v
+        is_lazy_list N v Skeys 1 Γ
         ∗
         ⌜ if b then key ∈ Skeys else key ∉ Skeys ⌝
       }}}.
     Proof.
-      iIntros (Φ) "#H HΦ".
-      iDestruct "H" as (head S) "(%Hequiv & %Hv & %Hmin & Hinv)".
+      iIntros (Φ) "H HΦ".
+      iDestruct "H" as (head S) "(%Hequiv & Hown & %Hv & %Hmin & #Hinv)".
       wp_lam. wp_let. rewrite -Hv.
-      wp_apply (find_spec head head key S).
-      { iSplit. done. iSplit. by iLeft. iPureIntro. lia. }
-      iIntros (pred succ) "(%Hrange' & %Hpred_in_S & %Hsucc_in_S & %Hkey_in_S & Hlock)".
+      wp_apply (find_spec1 with "[Hown]").
+      { iFrame "# ∗". iPureIntro; split. by left. lia. }
+      iIntros (pred succ) "(Hown & %Hkey_in_S)".
       wp_let. wp_match. wp_pures. wp_lam. wp_pures.
-      iModIntro.
 
-      case_bool_decide.
+      iModIntro; case_bool_decide.
       + iApply "HΦ". iSplit. 
-        iExists head, S. by iFrame "#".
+        iExists head, S. by iFrame "# ∗".
         iPureIntro. unfold key_equiv in Hequiv. 
-        apply elem_of_elements. rewrite Hequiv.
-        apply Hkey_in_S. congruence.
+        rewrite -elem_of_elements Hequiv Hkey_in_S.
+        congruence.
       + iApply "HΦ". iSplit. 
-        iExists head, S. by iFrame "#".
+        iExists head, S. by iFrame "# ∗".
         iPureIntro. intros Hin. 
-        apply elem_of_elements in Hin.
-        rewrite Hequiv in Hin. apply Hkey_in_S in Hin.
+        rewrite -elem_of_elements Hequiv Hkey_in_S in Hin.
         congruence.
     Qed.
-
-    Theorem findLock_spec (head curr: node_rep) (key: Z) (S: gset node_rep) :
+    
+    Theorem find_spec2 (head curr: node_rep) (key: Z) (γs γf: gname) :
       {{{ 
-        inv N (lazy_list_inv S head)
+        inv N (lazy_list_inv head γs γf)
         ∗
-        ⌜ curr = head ∨ curr ∈ S ⌝
+        (⌜ curr = head ⌝ ∨ own γs (◯ {[curr]}))
+        ∗
+        ⌜ node_key curr < key < INT_MAX ⌝
+      }}}
+      find (rep_to_node curr) #key
+      {{{ pred succ, RET SOMEV ((rep_to_node pred), (rep_to_node succ));
+        ⌜ node_key pred < key ≤ node_key succ ⌝
+        ∗
+        (⌜ pred = head ⌝ ∨ own γs (◯ {[pred]}))
+        ∗
+        (own γs (◯ {[succ]}) ∨ ⌜ succ = tail ⌝)
+        ∗
+        ∃ (l:loc) (γ: gname), ⌜ node_next pred = Some l ⌝ 
+                              ∗ 
+                              is_lock γ (node_lock pred) (node_inv l)
+      }}}.
+    Proof.
+      iIntros (Φ) "(#Hinv & Hown_curr & Hrange) HΦ".
+      iRevert (curr) "Hown_curr Hrange HΦ".
+      iLöb as "IH".
+      iIntros (curr) "#Hown_curr %Hrange HΦ".
+      wp_lam. wp_let. wp_lam. wp_pures.
+
+      destruct (node_next curr) as [l|] eqn:Hcurr_next; wp_pures.
+      + wp_bind (Load _).
+        iInv N as (S L) "(>%Hperm & >%Hsort & Hown_auth & Hown_frac & Hlist)" "Hclose".
+
+        iMod "Hown_auth".
+        iMod (own_update with "Hown_auth") as "[Hown_auth Hown_frag]".
+        { by apply auth_update_alloc, (gset_local_update S _ S). }
+
+        iAssert ((⌜ curr = head ∨ curr ∈ S ⌝)%I) with "[Hown_auth Hown_curr]" as %Hcurr_range.
+        {
+         iDestruct "Hown_curr" as "[Heq|Hown]"; first by iLeft.
+         iDestruct (own_valid_2 with "Hown_auth Hown") 
+          as %[Hvalid%gset_included]%auth_both_valid_discrete.
+         iPureIntro; right; set_solver.
+        }
+
+        rewrite (list_equiv_invert); last first.
+        { by rewrite -elem_of_list_In Hperm elem_of_elements. }
+        iDestruct "Hlist" as (succ l' γ) "(Hsucc_range & Hsome & Hpt & #Hlock & Himp)".
+        iMod "Hsucc_range" as %Hsucc_range;
+          rewrite -elem_of_list_In Hperm elem_of_elements in Hsucc_range.
+        iMod "Hsome" as %Hsome; assert (l = l') as <- by congruence.
+        iMod "Hpt"; wp_load.
+        iMod ("Hclose" with "[Hpt Himp Hown_auth Hown_frac]").
+        {
+          iNext. iExists S, L.
+          iPoseProof ("Himp" with "Hpt") as "Hlist".
+          by iFrame.
+        }
+
+        iModIntro. wp_let. wp_lam. wp_pures.
+        case_bool_decide as Hcase; wp_if.
+        - wp_pures. iApply "HΦ".
+          iModIntro; iFrame "#".
+
+          iSplit; first by (iPureIntro; lia).
+          iSplit.
+          { 
+            destruct Hsucc_range as [Hin|Heq]; last by iRight.
+            assert (S ≡ S ⋅ {[ succ ]}) as -> by set_solver.
+            iDestruct "Hown_frag" as "(? & ?)"; iLeft; iFrame.
+          }
+
+          iExists l, γ. by iFrame "#".
+        - iApply ("IH" $! succ with "[Hown_frag] [%]").
+          {
+            iRight.
+            assert (S ≡ S ⋅ {[ succ ]}) as ->.
+            {
+              destruct Hsucc_range as [Hin|Heq]; first set_solver.
+              subst; exfalso; rewrite /node_key/tail//= in Hcase; lia.
+            }
+            iDestruct "Hown_frag" as "(? & ?)"; iFrame.
+          }
+          { lia. }
+
+          iNext; iApply "HΦ".
+      + iInv N as (S L) "(>%Hperm & >%Hsort & Hown_auth & Hown_frac & Hlist)" "Hclose".
+
+        iMod "Hown_auth".
+        iAssert ((⌜ curr = head ∨ curr ∈ S ⌝)%I) with "[Hown_auth Hown_curr]" as %Hcurr_range.
+        {
+         iDestruct "Hown_curr" as "[Heq|Hown]"; first by iLeft.
+         iDestruct (own_valid_2 with "Hown_auth Hown") 
+          as %[Hvalid%gset_included]%auth_both_valid_discrete.
+         iPureIntro; right; set_solver.
+        }
+
+        rewrite (list_equiv_invert); last first.
+        { by rewrite -elem_of_list_In Hperm elem_of_elements. }
+        iDestruct "Hlist" as (succ l γ) "(Hsucc_range & Hsome & Hpt & #Hlock & Himp)".
+        iMod "Hsome" as %Hsome; congruence.
+    Qed.
+
+    Theorem findLock_spec (head curr: node_rep) (key: Z) (γs γf: gname) :
+      {{{ 
+        inv N (lazy_list_inv head γs γf)
+        ∗
+        (⌜ curr = head ⌝ ∨ own γs (◯ {[curr]}))
         ∗
         ⌜ node_key curr < key < INT_MAX ⌝
       }}}
@@ -292,9 +351,9 @@ Module LazyListSpec (Params: LAZY_LIST_PARAMS).
       {{{ pred succ, RET ((rep_to_node pred), (rep_to_node succ));
         ⌜ node_key pred < key ≤ node_key succ ⌝
         ∗
-        ⌜ pred = head ∨ pred ∈ S ⌝
+        (⌜ pred = head ⌝ ∨ own γs (◯ {[pred]}))
         ∗
-        ⌜ succ ∈ S ∨ succ = tail ⌝
+        (own γs (◯ {[succ]}) ∨ ⌜ succ = tail ⌝)
         ∗
         ∃ (l: loc) (γ: gname), ⌜ node_next pred = Some l ⌝
                                ∗
@@ -305,75 +364,72 @@ Module LazyListSpec (Params: LAZY_LIST_PARAMS).
                                locked γ
       }}}.
     Proof.
-      iIntros (Φ) "(#Hinv & Hcurr_range & Hrange) HΦ".
-      iRevert (curr) "Hcurr_range Hrange".
+      iIntros (Φ) "(#Hinv & Hown_curr & Hrange) HΦ".
+      iRevert (curr) "Hown_curr Hrange".
       iLöb as "IH". 
-      iIntros (curr) "%Hcurr_range %Hrange".
+      iIntros (curr) "#Hown_curr %Hrange".
+      
       wp_lam. wp_let.
-      wp_apply (find_spec head curr key S).
-      {  by iFrame "#". }
-      iIntros (pred succ) "(%Hrange' & %Hpred_in_S & %Hsucc_in_S & %Hkey_in_S & Hlock)".
+      wp_apply ((find_spec2 head curr key γs) with "[Hown_curr]").
+      { by iFrame "#". }
+      iIntros (pred succ) "(%Hrange' & #Hown_pred & #Hown_succ & Hlock)".
       iDestruct "Hlock" as (l γ) "(%Hsome & #Hlock)".
-      wp_pures. wp_lam.
-      wp_bind (Snd _).
-      iInv N as (L) "(>%Hperm & >%Hsort & Hlist)" "Hclose".
-      wp_pures.
-      iMod ("Hclose" with "[Hlist]").
-      { iNext; iExists L; by repeat iSplit. }
-      iModIntro.
+      wp_pures. wp_lam. wp_pures.
+
       wp_bind (acquire _).
       iApply (acquire_spec with "Hlock"); first done.
-      iNext. iIntros (v) "(Hnode & Hlocked)".
+      iNext; iIntros (v) "(Hnode & Hlocked)".
       wp_pures. wp_lam. wp_pures.
-      rewrite Hsome. wp_match.
+      rewrite Hsome; wp_match.
       iDestruct "Hnode" as (rep) "Hnode".
 
       wp_bind (Load _).
-      iInv N as (L') "(>%Hperm' & >%Hsort' & Hlist)" "Hclose".
-      assert (L = L') as <-.
+      iInv N as (S L) "(>%Hperm & >%Hsort & Hown_auth & Hown_frac & Hlist)" "Hclose".
+
+      iMod "Hown_auth".
+      iAssert ((⌜ pred = head ∨ pred ∈ S ⌝ ∗ ⌜succ ∈ S ∨ succ = tail⌝)%I) 
+        with "[Hown_auth Hown_pred Hown_succ]" as "(%Hpred_range & %Hsucc_range)".
       {
-        apply node_rep_sorted_eq.
-        + rewrite -app_ass in Hsort.
-          apply node_rep_sorted_app in Hsort; destruct Hsort as [Hsort ?].
-          apply node_rep_sorted_app in Hsort; by destruct Hsort.
-        + rewrite -app_ass in Hsort'.
-          apply node_rep_sorted_app in Hsort'; destruct Hsort' as [Hsort' ?].
-          apply node_rep_sorted_app in Hsort'; by destruct Hsort'.
-        + rewrite Hperm. by symmetry. 
+        iSplit.
+        - iDestruct "Hown_pred" as "[Heq|Hown]"; first by iLeft.
+          iDestruct (own_valid_2 with "Hown_auth Hown") 
+            as %[Hvalid%gset_included]%auth_both_valid_discrete.
+          iPureIntro; right; set_solver.
+        - iDestruct "Hown_succ" as "[Hown|Heq]"; last by iRight.
+          iDestruct (own_valid_2 with "Hown_auth Hown") 
+            as %[Hvalid%gset_included]%auth_both_valid_discrete.
+          iPureIntro; left; set_solver.
       }
+
       rewrite (list_equiv_invert L head pred); last first.
-      { by rewrite -elem_of_elements -Hperm elem_of_list_In -in_inv in Hpred_in_S. }
+      { by rewrite -elem_of_list_In Hperm elem_of_elements. }
       iDestruct "Hlist" as (succ' l' γ') "(>%Hsucc'_in_L & >%Hsome' & Hpt & _ & Himp)".
       assert (l = l') as <- by congruence.
 
       wp_load.
       iDestruct (mapsto_agree with "Hnode Hpt") as "%Hsucc"; rewrite Hsucc.
-      iMod ("Hclose" with "[Hpt Himp]").
+      iMod ("Hclose" with "[Hpt Himp Hown_auth Hown_frac]").
       {
-        iNext. iExists L.
-        iSplit. done.
-        iSplit. done.
-        iApply "Himp". iFrame.
+        iNext. iExists S, L.
+        iPoseProof ("Himp" with "Hpt") as "Hlist".
+        by iFrame.
       }
-      iModIntro.
-      
-      wp_let. repeat (wp_lam; wp_pures).
+
+      iModIntro. wp_let. wp_lam. wp_pures. wp_lam. wp_pures.
       case_bool_decide as Heq; wp_if.
-      + wp_pures. iApply "HΦ". iModIntro.
-        iSplit. done. iSplit. done. iSplit. done.
-        iExists l, γ. iSplit. done. iFrame; iFrame "#".
-        assert (succ = succ') as <-; last done.
+      + wp_pures. iApply "HΦ". iModIntro; iFrame "# ∗".
+        iSplit. done. iExists l, γ.
+        assert (succ = succ') as <-; last by iFrame "# ∗".
         apply (sorted_node_key_unique (L ++ [tail])).
         - apply node_rep_sorted_app in Hsort; by destruct Hsort.
-        - rewrite -elem_of_elements -Hperm elem_of_list_In in Hsucc_in_S.
-          by apply in_inv_rev. 
+        - by rewrite in_inv_rev -elem_of_list_In Hperm elem_of_elements.
         - by apply in_inv_rev. 
         - congruence.
       + wp_lam. wp_pures.
         wp_apply (release_spec with "[Hnode Hlocked]"); first done.
-        { iFrame; iFrame "#"; by iExists succ'. }
+        { iFrame "# ∗"; by iExists succ'. }
         iIntros. wp_pures.
-        iApply ("IH" with "HΦ"); auto.
+        by iApply ("IH" with "HΦ").
     Qed.
 
   End Proofs.
